Stateful SHA2_512: pass verification against HaCl integers

code/experimental/hash/Hacl.Hash.SHA2_512.fst
@@ -8,6 +8,7 @@ open FStar.Buffer
 
 open C.Loops
 
+open Hacl.Spec.Endianness
 open Hacl.Cast
 open Hacl.UInt8
 open Hacl.UInt32
@@ -138,26 +139,46 @@ private val constants_set_k:
 [@"substitute"]
 let constants_set_k k =
   Hacl.Utils.Experimental.hupd64_80 k
-  0x428a2f98d728ae22uL 0x7137449123ef65cduL 0xb5c0fbcfec4d3b2fuL 0xe9b5dba58189dbbcuL
-  0x3956c25bf348b538uL 0x59f111f1b605d019uL 0x923f82a4af194f9buL 0xab1c5ed5da6d8118uL
-  0xd807aa98a3030242uL 0x12835b0145706fbeuL 0x243185be4ee4b28cuL 0x550c7dc3d5ffb4e2uL
-  0x72be5d74f27b896fuL 0x80deb1fe3b1696b1uL 0x9bdc06a725c71235uL 0xc19bf174cf692694uL
-  0xe49b69c19ef14ad2uL 0xefbe4786384f25e3uL 0x0fc19dc68b8cd5b5uL 0x240ca1cc77ac9c65uL
-  0x2de92c6f592b0275uL 0x4a7484aa6ea6e483uL 0x5cb0a9dcbd41fbd4uL 0x76f988da831153b5uL
-  0x983e5152ee66dfabuL 0xa831c66d2db43210uL 0xb00327c898fb213fuL 0xbf597fc7beef0ee4uL
-  0xc6e00bf33da88fc2uL 0xd5a79147930aa725uL 0x06ca6351e003826fuL 0x142929670a0e6e70uL
-  0x27b70a8546d22ffcuL 0x2e1b21385c26c926uL 0x4d2c6dfc5ac42aeduL 0x53380d139d95b3dfuL
-  0x650a73548baf63deuL 0x766a0abb3c77b2a8uL 0x81c2c92e47edaee6uL 0x92722c851482353buL
-  0xa2bfe8a14cf10364uL 0xa81a664bbc423001uL 0xc24b8b70d0f89791uL 0xc76c51a30654be30uL
-  0xd192e819d6ef5218uL 0xd69906245565a910uL 0xf40e35855771202auL 0x106aa07032bbd1b8uL
-  0x19a4c116b8d2d0c8uL 0x1e376c085141ab53uL 0x2748774cdf8eeb99uL 0x34b0bcb5e19b48a8uL
-  0x391c0cb3c5c95a63uL 0x4ed8aa4ae3418acbuL 0x5b9cca4f7763e373uL 0x682e6ff3d6b2b8a3uL
-  0x748f82ee5defb2fcuL 0x78a5636f43172f60uL 0x84c87814a1f0ab72uL 0x8cc702081a6439ecuL
-  0x90befffa23631e28uL 0xa4506cebde82bde9uL 0xbef9a3f7b2c67915uL 0xc67178f2e372532buL
-  0xca273eceea26619cuL 0xd186b8c721c0c207uL 0xeada7dd6cde0eb1euL 0xf57d4f7fee6ed178uL
-  0x06f067aa72176fbauL 0x0a637dc5a2c898a6uL 0x113f9804bef90daeuL 0x1b710b35131c471buL
-  0x28db77f523047d84uL 0x32caab7b40c72493uL 0x3c9ebe0a15c9bebcuL 0x431d67c49c100d4cuL
-  0x4cc5d4becb3e42b6uL 0x597f299cfc657e2auL 0x5fcb6fab3ad6faecuL 0x6c44198c4a475817uL
+  (u64_to_h64 0x428a2f98d728ae22uL) (u64_to_h64 0x7137449123ef65cduL)
+  (u64_to_h64 0xb5c0fbcfec4d3b2fuL) (u64_to_h64 0xe9b5dba58189dbbcuL)
+  (u64_to_h64 0x3956c25bf348b538uL) (u64_to_h64 0x59f111f1b605d019uL)
+  (u64_to_h64 0x923f82a4af194f9buL) (u64_to_h64 0xab1c5ed5da6d8118uL)
+  (u64_to_h64 0xd807aa98a3030242uL) (u64_to_h64 0x12835b0145706fbeuL)
+  (u64_to_h64 0x243185be4ee4b28cuL) (u64_to_h64 0x550c7dc3d5ffb4e2uL)
+  (u64_to_h64 0x72be5d74f27b896fuL) (u64_to_h64 0x80deb1fe3b1696b1uL)
+  (u64_to_h64 0x9bdc06a725c71235uL) (u64_to_h64 0xc19bf174cf692694uL)
+  (u64_to_h64 0xe49b69c19ef14ad2uL) (u64_to_h64 0xefbe4786384f25e3uL)
+  (u64_to_h64 0x0fc19dc68b8cd5b5uL) (u64_to_h64 0x240ca1cc77ac9c65uL)
+  (u64_to_h64 0x2de92c6f592b0275uL) (u64_to_h64 0x4a7484aa6ea6e483uL)
+  (u64_to_h64 0x5cb0a9dcbd41fbd4uL) (u64_to_h64 0x76f988da831153b5uL)
+  (u64_to_h64 0x983e5152ee66dfabuL) (u64_to_h64 0xa831c66d2db43210uL)
+  (u64_to_h64 0xb00327c898fb213fuL) (u64_to_h64 0xbf597fc7beef0ee4uL)
+  (u64_to_h64 0xc6e00bf33da88fc2uL) (u64_to_h64 0xd5a79147930aa725uL)
+  (u64_to_h64 0x06ca6351e003826fuL) (u64_to_h64 0x142929670a0e6e70uL)
+  (u64_to_h64 0x27b70a8546d22ffcuL) (u64_to_h64 0x2e1b21385c26c926uL)
+  (u64_to_h64 0x4d2c6dfc5ac42aeduL) (u64_to_h64 0x53380d139d95b3dfuL)
+  (u64_to_h64 0x650a73548baf63deuL) (u64_to_h64 0x766a0abb3c77b2a8uL)
+  (u64_to_h64 0x81c2c92e47edaee6uL) (u64_to_h64 0x92722c851482353buL)
+  (u64_to_h64 0xa2bfe8a14cf10364uL) (u64_to_h64 0xa81a664bbc423001uL)
+  (u64_to_h64 0xc24b8b70d0f89791uL) (u64_to_h64 0xc76c51a30654be30uL)
+  (u64_to_h64 0xd192e819d6ef5218uL) (u64_to_h64 0xd69906245565a910uL)
+  (u64_to_h64 0xf40e35855771202auL) (u64_to_h64 0x106aa07032bbd1b8uL)
+  (u64_to_h64 0x19a4c116b8d2d0c8uL) (u64_to_h64 0x1e376c085141ab53uL)
+  (u64_to_h64 0x2748774cdf8eeb99uL) (u64_to_h64 0x34b0bcb5e19b48a8uL)
+  (u64_to_h64 0x391c0cb3c5c95a63uL) (u64_to_h64 0x4ed8aa4ae3418acbuL)
+  (u64_to_h64 0x5b9cca4f7763e373uL) (u64_to_h64 0x682e6ff3d6b2b8a3uL)
+  (u64_to_h64 0x748f82ee5defb2fcuL) (u64_to_h64 0x78a5636f43172f60uL)
+  (u64_to_h64 0x84c87814a1f0ab72uL) (u64_to_h64 0x8cc702081a6439ecuL)
+  (u64_to_h64 0x90befffa23631e28uL) (u64_to_h64 0xa4506cebde82bde9uL)
+  (u64_to_h64 0xbef9a3f7b2c67915uL) (u64_to_h64 0xc67178f2e372532buL)
+  (u64_to_h64 0xca273eceea26619cuL) (u64_to_h64 0xd186b8c721c0c207uL)
+  (u64_to_h64 0xeada7dd6cde0eb1euL) (u64_to_h64 0xf57d4f7fee6ed178uL)
+  (u64_to_h64 0x06f067aa72176fbauL) (u64_to_h64 0x0a637dc5a2c898a6uL)
+  (u64_to_h64 0x113f9804bef90daeuL) (u64_to_h64 0x1b710b35131c471buL)
+  (u64_to_h64 0x28db77f523047d84uL) (u64_to_h64 0x32caab7b40c72493uL)
+  (u64_to_h64 0x3c9ebe0a15c9bebcuL) (u64_to_h64 0x431d67c49c100d4cuL)
+  (u64_to_h64 0x4cc5d4becb3e42b6uL) (u64_to_h64 0x597f299cfc657e2auL)
+  (u64_to_h64 0x5fcb6fab3ad6faecuL) (u64_to_h64 0x6c44198c4a475817uL)
 
 
 #reset-options " --max_fuel 0 --z3rlimit 10"
@@ -174,11 +195,11 @@ val constants_set_h_0:
 [@"substitute"]
 let constants_set_h_0 hash =
   Hacl.Utils.Experimental.hupd64_8 hash
-  0x6a09e667f3bcc908uL 0xbb67ae8584caa73buL 0x3c6ef372fe94f82buL 0xa54ff53a5f1d36f1uL
-  0x510e527fade682d1uL 0x9b05688c2b3e6c1fuL 0x1f83d9abfb41bd6buL 0x5be0cd19137e2179uL
+  (u64_to_h64 0x6a09e667f3bcc908uL) (u64_to_h64 0xbb67ae8584caa73buL) (u64_to_h64 0x3c6ef372fe94f82buL) (u64_to_h64 0xa54ff53a5f1d36f1uL)
+  (u64_to_h64 0x510e527fade682d1uL) (u64_to_h64 0x9b05688c2b3e6c1fuL) (u64_to_h64 0x1f83d9abfb41bd6buL) (u64_to_h64 0x5be0cd19137e2179uL)
 
 
-#reset-options " --max_fuel 0 --z3rlimit 10"
+#reset-options " --max_fuel 0 --z3rlimit 20"
 
 [@ "substitute"]
 private
@@ -188,19 +209,19 @@ val ws_part_1_core:
   i:UInt32.t{UInt32.v i < 16} ->
   Stack unit
         (requires (fun h -> live h ws_w /\ live h block_w /\
-          (let seq_ws = as_seq h ws_w in
-           let seq_block = as_seq h block_w in
+          (let seq_ws = reveal_h64s (as_seq h ws_w) in
+           let seq_block = reveal_h64s (as_seq h block_w) in
            (forall (j:nat). {:pattern (Seq.index seq_ws j)} j < UInt32.v i ==> Seq.index seq_ws j == Spec.ws seq_block j))
         ))
         (ensures  (fun h0 r h1 -> live h1 ws_w /\ live h0 ws_w
                   /\ live h1 block_w /\ live h0 block_w /\ modifies_1 ws_w h0 h1 /\
                   as_seq h1 block_w == as_seq h0 block_w
-                  /\ (let w = as_seq h1 ws_w in
-                  let b = as_seq h0 block_w in
+                  /\ (let w = reveal_h64s (as_seq h1 ws_w) in
+                  let b = reveal_h64s (as_seq h0 block_w) in
                   (forall (j:nat). {:pattern (Seq.index w j)} j < UInt32.v i+1 ==> Seq.index w j == Spec.ws b j))))
 
 
-#reset-options " --max_fuel 0 --z3rlimit 10"
+#reset-options " --max_fuel 0 --z3rlimit 20"
 
 private
 val lemma_spec_ws_def:
@@ -208,7 +229,7 @@ val lemma_spec_ws_def:
   i:nat{i < 16} ->
   Lemma (Spec.ws b i == Seq.index b i)
 
-#reset-options " --max_fuel 1 --z3rlimit 10"
+#reset-options " --max_fuel 1 --z3rlimit 20"
 
 let lemma_spec_ws_def b i = ()
 
@@ -222,8 +243,8 @@ let ws_part_1_core ws_w block_w t =
     let h1 = ST.get() in
     let h' = ST.get() in
     no_upd_lemma_1 h0 h1 ws_w block_w;
-    lemma_spec_ws_def (as_seq h block_w) (UInt32.v t);
-    assert(Seq.index (as_seq h1 ws_w) (UInt32.v t) == Seq.index (as_seq h block_w) (UInt32.v t))
+    lemma_spec_ws_def (reveal_h64s (as_seq h block_w)) (UInt32.v t);
+    assert(Seq.index (reveal_h64s (as_seq h1 ws_w)) (UInt32.v t) == Seq.index (reveal_h64s(as_seq h block_w)) (UInt32.v t))
 
 
 val lemma_modifies_0_is_modifies_1:
@@ -243,8 +264,8 @@ private val ws_part_1:
         (requires (fun h -> live h ws_w /\ live h block_w))
         (ensures  (fun h0 r h1 -> live h1 ws_w /\ live h0 ws_w
                   /\ live h1 block_w /\ live h0 block_w /\ modifies_1 ws_w h0 h1
-                  /\ (let w = as_seq h1 ws_w in
-                  let b = as_seq h0 block_w in
+                  /\ (let w = reveal_h64s (as_seq h1 ws_w) in
+                  let b = reveal_h64s (as_seq h0 block_w) in
                   (forall (i:nat). {:pattern (Seq.index w i)} i < 16 ==> Seq.index w i == Spec.ws b i))))
 
 #reset-options " --max_fuel 0 --z3rlimit 200"
@@ -255,8 +276,8 @@ let ws_part_1 ws_w block_w =
   let inv (h1: HS.mem) (i: nat) : Type0 =
     i <= 16 /\ live h1 ws_w /\ live h1 block_w /\ modifies_1 ws_w h0 h1 /\
     as_seq h1 block_w == as_seq h0 block_w
-    /\ (let seq_block = as_seq h0 block_w in
-       let w = as_seq h1 ws_w in
+    /\ (let seq_block = reveal_h64s (as_seq h0 block_w) in
+       let w = reveal_h64s (as_seq h1 ws_w) in
     (forall (j:nat). {:pattern (Seq.index w j)} j < i ==> Seq.index w j == Spec.ws seq_block j))
   in
   let f' (t:uint32_t {v t < 16}) :
@@ -271,7 +292,7 @@ let ws_part_1 ws_w block_w =
   let h1 = ST.get() in ()
 
 
-#reset-options " --max_fuel 0 --z3rlimit 10"
+#reset-options " --max_fuel 0 --z3rlimit 20"
 
 [@ "substitute"]
 private
@@ -281,18 +302,18 @@ val ws_part_2_core:
   i:UInt32.t{16 <= UInt32.v i /\ UInt32.v i < 80} ->
   Stack unit
         (requires (fun h -> live h ws_w /\ live h block_w /\
-                  (let w = as_seq h ws_w in
-                  let b = as_seq h block_w in
+                  (let w = reveal_h64s (as_seq h ws_w) in
+                  let b = reveal_h64s (as_seq h block_w) in
                   (forall (j:nat). {:pattern (Seq.index w j)} j < UInt32.v i ==> Seq.index w j == Spec.ws b j))))
         (ensures  (fun h0 r h1 -> live h1 ws_w /\ live h0 ws_w
                   /\ live h1 block_w /\ live h0 block_w /\ modifies_1 ws_w h0 h1 /\
-                  as_seq h1 block_w == as_seq h0 block_w
-                  /\ (let w = as_seq h1 ws_w in
-                  let b = as_seq h0 block_w in
+                  reveal_h64s (as_seq h1 block_w) == reveal_h64s (as_seq h0 block_w)
+                  /\ (let w = reveal_h64s (as_seq h1 ws_w) in
+                  let b = reveal_h64s (as_seq h0 block_w) in
                   (forall (j:nat). {:pattern (Seq.index w j)} j < UInt32.v i+1 ==> Seq.index w j == Spec.ws b j))))
 
 
-#reset-options " --max_fuel 1 --z3rlimit 10"
+#reset-options " --max_fuel 1 --z3rlimit 20"
 
 private
 val lemma_spec_ws_def2:
@@ -302,11 +323,11 @@ val lemma_spec_ws_def2:
         let t15 = Spec.ws b (t - 15) in
         let t7  = Spec.ws b (t - 7) in
         let t2  = Spec.ws b (t - 2) in
-        let s1 = _sigma1 t2 in
-        let s0 = _sigma0 t15 in
+        let s1 = Spec._sigma1 t2 in
+        let s0 = Spec._sigma0 t15 in
         Spec.ws b t == FStar.UInt64.(s1 +%^ (t7 +%^ (s0 +%^ t16))))
 
-#reset-options " --max_fuel 1 --z3rlimit 10"
+#reset-options " --max_fuel 1 --z3rlimit 20"
 
 let lemma_spec_ws_def2 b i = ()
 
@@ -322,11 +343,11 @@ let ws_part_2_core ws_w block_w t =
     ws_w.(t) <- H64.((_sigma1 t2) +%^ (t7 +%^ ((_sigma0 t15) +%^ t16)));
     let h1 = ST.get () in
     no_upd_lemma_1 h0 h1 ws_w block_w;
-    lemma_spec_ws_def2 (as_seq h0 block_w) (UInt32.v t);
-    assert(Seq.index (as_seq h1 ws_w) (UInt32.v t) == Spec.ws (as_seq h0 block_w) (UInt32.v t))
+    lemma_spec_ws_def2 (reveal_h64s (as_seq h0 block_w)) (UInt32.v t);
+    assert(Seq.index (reveal_h64s (as_seq h1 ws_w)) (UInt32.v t) == Spec.ws (reveal_h64s (as_seq h0 block_w)) (UInt32.v t))
 
 
-#reset-options " --max_fuel 0 --z3rlimit 10"
+#reset-options " --max_fuel 0 --z3rlimit 20"
 
 [@"substitute"]
 private val ws_part_2:
@@ -334,13 +355,13 @@ private val ws_part_2:
   block_w :uint64_p {length block_w = v size_block_w /\ disjoint ws_w block_w} ->
   Stack unit
         (requires (fun h -> live h ws_w /\ live h block_w
-                  /\ (let w = as_seq h ws_w in
-                  let b = as_seq h block_w in
+                  /\ (let w = reveal_h64s (as_seq h ws_w) in
+                  let b = reveal_h64s (as_seq h block_w) in
                   (forall (i:nat). {:pattern (Seq.index w i)} i < 16 ==> Seq.index w i == Spec.ws b i))))
         (ensures  (fun h0 r h1 -> live h1 ws_w /\ live h0 ws_w
                   /\ live h1 block_w /\ live h0 block_w /\ modifies_1 ws_w h0 h1
-                  /\ (let w = as_seq h1 ws_w in
-                  let b = as_seq h0 block_w in
+                  /\ (let w = reveal_h64s (as_seq h1 ws_w) in
+                  let b = reveal_h64s (as_seq h0 block_w) in
                   (forall (i:nat). {:pattern (Seq.index w i)} i < 80 ==> Seq.index w i == Spec.ws b i))))
 
 #reset-options " --max_fuel 0 --z3rlimit 200"
@@ -350,9 +371,9 @@ let ws_part_2 ws_w block_w =
   let h0 = ST.get() in
   let inv (h1: HS.mem) (i: nat) : Type0 =
     live h1 ws_w /\ live h1 block_w /\ modifies_1 ws_w h0 h1 /\ 16 <= i /\ i <= 80
-    /\ as_seq h1 block_w == as_seq h0 block_w
-    /\ (let seq_block = as_seq h0 block_w in
-       let w = as_seq h1 ws_w in
+    /\ reveal_h64s (as_seq h1 block_w) == reveal_h64s (as_seq h0 block_w)
+    /\ (let seq_block = reveal_h64s (as_seq h0 block_w) in
+       let w = reveal_h64s (as_seq h1 ws_w) in
     (forall (j:nat). {:pattern (Seq.index w j)} j < i ==> Seq.index w j == Spec.ws seq_block j))
   in
   let f' (t:uint32_t {16 <= v t /\ v t < v size_ws_w}) :
@@ -367,7 +388,7 @@ let ws_part_2 ws_w block_w =
   let h1 = ST.get() in ()
 
 
-#reset-options "--max_fuel 0  --z3rlimit 10"
+#reset-options "--max_fuel 0  --z3rlimit 20"
 
 [@"substitute"]
 private val ws:
@@ -377,11 +398,11 @@ private val ws:
         (requires (fun h -> live h ws_w /\ live h block_w))
         (ensures  (fun h0 r h1 -> live h1 ws_w /\ live h0 ws_w
                   /\ live h1 block_w /\ live h0 block_w /\ modifies_1 ws_w h0 h1
-                  /\ (let w = as_seq h1 ws_w in
-                  let b = as_seq h0 block_w in
+                  /\ (let w = reveal_h64s (as_seq h1 ws_w) in
+                  let b = reveal_h64s (as_seq h0 block_w) in
                   (forall (i:nat). {:pattern (Seq.index w i)} i < 80 ==> Seq.index w i == Spec.ws b i))))
 
-#reset-options "--max_fuel 0  --z3rlimit 20"
+#reset-options "--max_fuel 0  --z3rlimit 50"
 
 [@"substitute"]
 let ws ws_w block_w =
@@ -389,7 +410,7 @@ let ws ws_w block_w =
   ws_part_2 ws_w block_w
 
 
-#reset-options "--max_fuel 0  --z3rlimit 10"
+#reset-options "--max_fuel 0  --z3rlimit 20"
 
 [@"substitute"]
 private val shuffle_core:
@@ -400,15 +421,15 @@ private val shuffle_core:
   t      :uint32_t {v t < v size_k_w} ->
   Stack unit
         (requires (fun h -> live h hash_w /\ live h ws_w /\ live h k_w /\ live h block_w /\
-          as_seq h k_w == Spec.k /\
-          (let w = as_seq h ws_w in
-           let b = as_seq h block_w in
+          reveal_h64s (as_seq h k_w) == Spec.k /\
+          (let w = reveal_h64s (as_seq h ws_w) in
+           let b = reveal_h64s (as_seq h block_w) in
            (forall (i:nat). {:pattern (Seq.index w i)} i < 80 ==> Seq.index w i == Spec.ws b i)) ))
         (ensures  (fun h0 r h1 -> live h0 hash_w /\ live h0 ws_w /\ live h0 k_w /\ live h0 block_w
           /\ live h1 hash_w /\ modifies_1 hash_w h0 h1
-                  /\ (let seq_hash_0 = as_seq h0 hash_w in
-                  let seq_hash_1 = as_seq h1 hash_w in
-                  let seq_block = as_seq h0 block_w in
+                  /\ (let seq_hash_0 = reveal_h64s (as_seq h0 hash_w) in
+                  let seq_hash_1 = reveal_h64s (as_seq h1 hash_w) in
+                  let seq_block = reveal_h64s (as_seq h0 block_w) in
                   seq_hash_1 == Spec.shuffle_core seq_block seq_hash_0 (U32.v t))))
 
 #reset-options "--max_fuel 0  --z3rlimit 100"
@@ -434,7 +455,7 @@ let shuffle_core hash block ws k t =
   Utils.hupd64_8 hash H64.(t1 +%^ t2) a b c H64.(d +%^ t1) e f g
 
 
-#reset-options "--max_fuel 0  --z3rlimit 10"
+#reset-options "--max_fuel 0  --z3rlimit 20"
 
 [@"substitute"]
 private val shuffle:
@@ -444,15 +465,15 @@ private val shuffle:
   k_w    :uint64_p {length k_w = v size_k_w /\ disjoint k_w hash_w} ->
   Stack unit
         (requires (fun h -> live h hash_w /\ live h ws_w /\ live h k_w /\ live h block_w /\
-          as_seq h k_w == Spec.k /\
-          (let w = as_seq h ws_w in
-           let b = as_seq h block_w in
+          reveal_h64s (as_seq h k_w) == Spec.k /\
+          (let w = reveal_h64s (as_seq h ws_w) in
+           let b = reveal_h64s (as_seq h block_w) in
            (forall (i:nat). {:pattern (Seq.index w i)} i < 80 ==> Seq.index w i == Spec.ws b i)) ))
         (ensures  (fun h0 r h1 -> live h1 hash_w /\ modifies_1 hash_w h0 h1 /\ live h0 block_w
                   /\ live h0 hash_w
-                  /\ (let seq_hash_0 = as_seq h0 hash_w in
-                  let seq_hash_1 = as_seq h1 hash_w in
-                  let seq_block = as_seq h0 block_w in
+                  /\ (let seq_hash_0 = reveal_h64s (as_seq h0 hash_w) in
+                  let seq_hash_1 = reveal_h64s (as_seq h1 hash_w) in
+                  let seq_block = reveal_h64s (as_seq h0 block_w) in
                   seq_hash_1 == Spec.shuffle seq_hash_0 seq_block)))
 
 #reset-options "--max_fuel 0  --z3rlimit 100"
@@ -462,8 +483,8 @@ let shuffle hash block ws k =
   let h0 = ST.get() in
   let inv (h1: HS.mem) (i: nat) : Type0 =
     live h1 hash /\ modifies_1 hash h0 h1 /\ i <= v size_ws_w
-    /\ (let seq_block = as_seq h0 block in
-    as_seq h1 hash == repeat_range_spec 0 i (Spec.shuffle_core seq_block) (as_seq h0 hash))
+    /\ (let seq_block = reveal_h64s (as_seq h0 block) in
+    reveal_h64s (as_seq h1 hash) == repeat_range_spec 0 i (Spec.shuffle_core seq_block) (reveal_h64s (as_seq h0 hash)))
   in
   let f' (t:uint32_t {v t < v size_ws_w}) :
     Stack unit
@@ -471,9 +492,9 @@ let shuffle hash block ws k =
       (ensures (fun h_1 _ h_2 -> inv h_2 (UInt32.v t + 1)))
     =
     shuffle_core hash block ws k t;
-    C.Loops.lemma_repeat_range_spec 0 (UInt32.v t + 1) (Spec.shuffle_core (as_seq h0 block)) (as_seq h0 hash)
+    C.Loops.lemma_repeat_range_spec 0 (UInt32.v t + 1) (Spec.shuffle_core (reveal_h64s (as_seq h0 block))) (reveal_h64s (as_seq h0 hash))
   in
-  C.Loops.lemma_repeat_range_0 0 0 (Spec.shuffle_core (as_seq h0 block)) (as_seq h0 hash);
+  C.Loops.lemma_repeat_range_0 0 0 (Spec.shuffle_core (reveal_h64s (as_seq h0 block))) (reveal_h64s (as_seq h0 hash));
   for 0ul size_ws_w inv f'
 
 
@@ -486,9 +507,9 @@ private val sum_hash:
   Stack unit
     (requires (fun h -> live h hash_0 /\ live h hash_1))
     (ensures  (fun h0 _ h1 -> live h0 hash_0 /\ live h1 hash_0 /\ live h0 hash_1 /\ modifies_1 hash_0 h0 h1
-              /\ (let new_seq_hash_0 = as_seq h1 hash_0 in
-              let seq_hash_0 = as_seq h0 hash_0 in
-              let seq_hash_1 = as_seq h0 hash_1 in
+              /\ (let new_seq_hash_0 = reveal_h64s (as_seq h1 hash_0) in
+              let seq_hash_0 = reveal_h64s (as_seq h0 hash_0) in
+              let seq_hash_1 = reveal_h64s (as_seq h0 hash_1) in
               let res        = Spec.Loops.seq_map2 (fun x y -> FStar.UInt64.(x +%^ y)) seq_hash_0 seq_hash_1 in
               new_seq_hash_0 == res)))
 
@@ -497,11 +518,11 @@ let sum_hash hash_0 hash_1 =
   let h0 = ST.get() in
   C.Loops.in_place_map2 hash_0 hash_1 size_hash_w (fun x y -> H64.(x +%^ y));
   let h1 = ST.get() in
-  Seq.lemma_eq_intro (Spec.Loops.seq_map2 (fun x y -> FStar.UInt64.(x +%^ y)) (as_seq h0 hash_0) (as_seq  h0 hash_1)) (as_seq h1 hash_0)
+  Seq.lemma_eq_intro (Spec.Loops.seq_map2 (fun x y -> FStar.UInt64.(x +%^ y)) (reveal_h64s (as_seq h0 hash_0)) (reveal_h64s (as_seq  h0 hash_1))) (reveal_h64s (as_seq h1 hash_0))
 
 
 
-#reset-options "--max_fuel 0  --z3rlimit 10"
+#reset-options "--max_fuel 0  --z3rlimit 20"
 
 [@"c_inline"]
 val alloc:
@@ -566,7 +587,7 @@ let copy_hash hash_w_1 hash_w_2 =
   Lemmas.lemma_blit_slices_eq h0 h1 hash_w_1 hash_w_2 (v size_hash_w)
 
 
-#reset-options "--max_fuel 0  --z3rlimit 10"
+#reset-options "--max_fuel 0  --z3rlimit 20"
 
 [@"substitute"]
 private val update_core:
@@ -577,15 +598,15 @@ private val update_core:
   k_w    :uint64_p {length k_w = v size_k_w /\ disjoint k_w hash_w} ->
   Stack unit
         (requires (fun h0 -> live h0 hash_w /\ live h0 data /\ live h0 data_w /\ live h0 ws_w /\ live h0 k_w
-                  /\ as_seq h0 k_w == Spec.k
-                  /\ (as_seq h0 data_w = Spec.Lib.uint64s_from_be (v size_block_w) (as_seq h0 data))
-                  /\ (let w = as_seq h0 ws_w in
-                  let b = as_seq h0 data_w in
+                  /\ reveal_h64s (as_seq h0 k_w) == Spec.k
+                  /\ (reveal_h64s (as_seq h0 data_w) = Spec.Lib.uint64s_from_be (v size_block_w) (reveal_sbytes (as_seq h0 data)))
+                  /\ (let w = reveal_h64s (as_seq h0 ws_w) in
+                  let b = reveal_h64s (as_seq h0 data_w) in
                   (forall (i:nat). {:pattern (Seq.index w i)} i < 80 ==> Seq.index w i == Spec.ws b i))))
         (ensures  (fun h0 r h1 -> live h0 hash_w /\ live h0 data /\ live h0 data_w /\ live h1 hash_w /\ modifies_1 hash_w h0 h1
-                  /\ (let seq_hash_0 = as_seq h0 hash_w in
-                  let seq_hash_1 = as_seq h1 hash_w in
-                  let seq_block = as_seq h0 data in
+                  /\ (let seq_hash_0 = reveal_h64s (as_seq h0 hash_w) in
+                  let seq_hash_1 = reveal_h64s (as_seq h1 hash_w) in
+                  let seq_block = reveal_sbytes (as_seq h0 data) in
                   let res = Spec.update seq_hash_0 seq_block in
                   seq_hash_1 == res)))
 
@@ -604,8 +625,8 @@ let update_core hash_w data data_w ws_w k_w =
 
   let h1 = ST.get() in
 
-  assert(  let b = Spec.words_from_be Spec.size_block_w (as_seq h0 data) in
-           as_seq h0 data_w == b);
+  assert(  let b = Spec.words_from_be Spec.size_block_w (reveal_sbytes (as_seq h0 data)) in
+           reveal_h64s (as_seq h0 data_w) == b);
 
   (* Allocate space for converting the data block *)
   let hash_0 = Buffer.create (u64_to_h64 0uL) size_hash_w in
@@ -634,10 +655,10 @@ let update_core hash_w data data_w ws_w k_w =
   shuffle hash_0 data_w ws_w k_w;
 
   let h4 = ST.get() in
-  assert(let b = Spec.words_from_be Spec.size_block_w (as_seq h0 data) in
-         let ha = Spec.shuffle (as_seq h0 hash_w) b in
+  assert(let b = Spec.words_from_be Spec.size_block_w (reveal_sbytes (as_seq h0 data)) in
+         let ha = Spec.shuffle (reveal_h64s (as_seq h0 hash_w)) b in
          as_seq h4 hash_w == as_seq h0 hash_w /\
-         as_seq h4 hash_0 == ha);
+         reveal_h64s (as_seq h4 hash_0) == ha);
 
   no_upd_lemma_1 h3 h4 hash_0 data;
   no_upd_lemma_1 h3 h4 hash_0 data_w;
@@ -650,14 +671,14 @@ let update_core hash_w data data_w ws_w k_w =
 
   let h5 = ST.get() in
 
-   assert(let x = as_seq h4 hash_w in
-          let y = as_seq h4 hash_0 in
-          x == as_seq h0 hash_w /\
-          y == Spec.shuffle (as_seq h0 hash_w) (Spec.words_from_be Spec.size_block_w (as_seq h0 data)));
+   assert(let x = reveal_h64s (as_seq h4 hash_w) in
+          let y = reveal_h64s (as_seq h4 hash_0) in
+          x == reveal_h64s (as_seq h0 hash_w) /\
+          y == Spec.shuffle (reveal_h64s (as_seq h0 hash_w)) (Spec.words_from_be Spec.size_block_w (reveal_sbytes (as_seq h0 data))));
 
-  assert(let x = as_seq h0 hash_w in
-         let y = Spec.shuffle (as_seq h0 hash_w) (Spec.words_from_be Spec.size_block_w (as_seq h0 data)) in
-         let z = as_seq h5 hash_w in
+  assert(let x = reveal_h64s (as_seq h0 hash_w) in
+         let y = Spec.shuffle (reveal_h64s (as_seq h0 hash_w)) (Spec.words_from_be Spec.size_block_w (reveal_sbytes (as_seq h0 data))) in
+         let z = reveal_h64s (as_seq h5 hash_w) in
          let z' = Spec.Loops.seq_map2 (fun x y -> FStar.UInt64.(x +%^ y)) x y in
          z == z');
 
@@ -680,7 +701,7 @@ val update:
                   /\ (let seq_k = Seq.slice (as_seq h0 state) (U32.v pos_k_w) (U32.(v pos_k_w + v size_k_w)) in
                   let seq_counter = Seq.slice (as_seq h0 state) (U32.v pos_count_w) (U32.(v pos_count_w + v size_count_w)) in
                   let counter = Seq.index seq_counter 0 in
-                  seq_k == Spec.k /\ H64.v counter < (pow2 64 - 1))))
+                  reveal_h64s seq_k == Spec.k /\ H64.v counter < (pow2 64 - 1))))
         (ensures  (fun h0 r h1 -> live h0 state /\ live h0 data /\ live h1 state /\ modifies_1 state h0 h1
                   /\ (let seq_hash_0 = Seq.slice (as_seq h0 state) (U32.v pos_whash_w) (U32.(v pos_whash_w + v size_whash_w)) in
                   let seq_hash_1 = Seq.slice (as_seq h1 state) (U32.v pos_whash_w) (U32.(v pos_whash_w + v size_whash_w)) in
@@ -693,7 +714,7 @@ val update:
                   let counter_1 = Seq.index seq_counter_1 0 in
                   seq_k_0 == seq_k_1
                   /\ H64.v counter_1 = H64.v counter_0 + 1 /\ H64.v counter_1 < pow2 64
-                  /\ seq_hash_1 == Spec.update seq_hash_0 seq_block)))
+                  /\ reveal_h64s seq_hash_1 == Spec.update (reveal_h64s seq_hash_0) (reveal_sbytes seq_block))))
 
 #reset-options "--max_fuel 0  --z3rlimit 200"
 
@@ -742,7 +763,7 @@ val update_multi:
                   /\ (let seq_k = Seq.slice (as_seq h0 state) (U32.v pos_k_w) (U32.(v pos_k_w + v size_k_w)) in
                   let seq_counter = Seq.slice (as_seq h0 state) (U32.v pos_count_w) (U32.(v pos_count_w + v size_count_w)) in
                   let counter = Seq.index seq_counter 0 in
-                  seq_k == Spec.k /\ H64.v counter < (pow2 64 - (v n)))))
+                  reveal_h64s seq_k == Spec.k /\ H64.v counter < (pow2 64 - (v n)))))
         (ensures  (fun h0 _ h1 -> live h0 state /\ live h0 data /\ live h1 state /\ modifies_1 state h0 h1
                   /\ (let seq_hash_0 = Seq.slice (as_seq h0 state) (U32.v pos_whash_w) (U32.(v pos_whash_w + v size_whash_w)) in
                   let seq_hash_1 = Seq.slice (as_seq h1 state) (U32.v pos_whash_w) (U32.(v pos_whash_w + v size_whash_w)) in
@@ -755,7 +776,7 @@ val update_multi:
                   let counter_1 = Seq.index seq_counter_1 0 in
                   seq_k_0 == seq_k_1
                   /\ H64.v counter_1 = H64.v counter_0 + (v n) /\ H64.v counter_1 < pow2 64
-                  /\ seq_hash_1 == Spec.update_multi seq_hash_0 seq_blocks)))
+                  /\ reveal_h64s seq_hash_1 == Spec.update_multi (reveal_h64s seq_hash_0) (reveal_sbytes seq_blocks))))
 
 #reset-options "--max_fuel 0  --z3rlimit 200"
 
@@ -766,14 +787,14 @@ let rec update_multi state data n =
     Lemmas.lemma_aux_1 (v n) (v size_block);
     assert (length data = 0);
     Lemmas.lemma_modifies_0_is_modifies_1 h0 state;
-    Lemmas.lemma_update_multi_def (Seq.slice (as_seq h0 state) (U32.v pos_whash_w) (U32.(v pos_whash_w + v size_whash_w))) (as_seq h0 data)
+    Lemmas.lemma_update_multi_def (reveal_h64s (Seq.slice (as_seq h0 state) (U32.v pos_whash_w) (U32.(v pos_whash_w + v size_whash_w)))) (reveal_sbytes (as_seq h0 data))
   )
   else
     begin
     assert(v n > 0);
     Lemmas.lemma_aux_2 (v n) (v size_block);
     assert(length data > 0);
-    Lemmas.lemma_update_multi_def (Seq.slice (as_seq h0 state) (U32.v pos_whash_w) (U32.(v pos_whash_w + v size_whash_w))) (as_seq h0 data);
+    Lemmas.lemma_update_multi_def (reveal_h64s (Seq.slice (as_seq h0 state) (U32.v pos_whash_w) (U32.(v pos_whash_w + v size_whash_w)))) (reveal_sbytes (as_seq h0 data));
 
     (* Get the current block for the data *)
     let b = Buffer.sub data 0ul size_block in
@@ -816,7 +837,7 @@ val set_pad_part1:
   Stack unit
         (requires (fun h0 -> live h0 buf1))
         (ensures  (fun h0 _ h1 -> live h0 buf1 /\ live h1 buf1 /\ modifies_1 buf1 h0 h1
-                             /\ (let seq_buf1 = as_seq h1 buf1 in
+                             /\ (let seq_buf1 = reveal_sbytes (as_seq h1 buf1) in
                              seq_buf1 = Seq.create 1 0x80uy)))
 
 #reset-options "--max_fuel 0 --z3rlimit 100"
@@ -825,7 +846,7 @@ val set_pad_part1:
 let set_pad_part1 buf1 =
   Buffer.upd buf1 0ul (u8_to_h8 0x80uy);
   let h = ST.get () in
-  Seq.lemma_eq_intro (as_seq h buf1) (Seq.create 1 0x80uy)
+  Seq.lemma_eq_intro (reveal_sbytes (as_seq h buf1)) (Seq.create 1 0x80uy)
 
 
 #reset-options "--max_fuel 0  --z3rlimit 20"
@@ -837,7 +858,7 @@ val set_pad_part2:
   Stack unit
         (requires (fun h0 -> live h0 buf2))
         (ensures  (fun h0 _ h1 -> live h0 buf2 /\ live h1 buf2 /\ modifies_1 buf2 h0 h1
-                  /\ (let seq_buf2 = as_seq h1 buf2 in
+                  /\ (let seq_buf2 = reveal_sbytes (as_seq h1 buf2) in
                   seq_buf2 == Endianness.big_bytes size_len_8 (H128.v encodedlen))))
 
 #reset-options "--max_fuel 0  --z3rlimit 30"
@@ -861,10 +882,10 @@ val pad:
                      /\ (length padding + U64.v len) % v size_block = 0} ->
   Stack unit
         (requires (fun h0 -> live h0 padding
-                  /\ (let seq_padding = as_seq h0 padding in
+                  /\ (let seq_padding = reveal_sbytes (as_seq h0 padding) in
                   seq_padding == Seq.create (1 + Spec.pad0_length (U64.v len) + v size_len_8) 0uy )))
         (ensures  (fun h0 _ h1 -> live h0 padding /\ live h1 padding /\ modifies_1 padding h0 h1
-                  /\ (let seq_padding = as_seq h1 padding in
+                  /\ (let seq_padding = reveal_sbytes (as_seq h1 padding) in
                   seq_padding == Spec.pad (H64.v n * v size_block) (U64.v len))))
 
 #reset-options "--max_fuel 0  --z3rlimit 100"
@@ -884,8 +905,8 @@ let pad padding n len =
   let encodedlen = encode_length n len in
 
   (**) let h0 = ST.get () in
-  (**) Seq.lemma_eq_intro (as_seq h0 zeros) (Seq.create (v pad0len) 0uy);
-  (**) assert(as_seq h0 zeros == Seq.create (v pad0len) 0uy);
+  (**) Seq.lemma_eq_intro (reveal_sbytes (as_seq h0 zeros)) (Seq.create (v pad0len) 0uy);
+  (**) assert(reveal_sbytes (as_seq h0 zeros) == Seq.create (v pad0len) 0uy);
 
   (* Set the first byte of the padding *)
   set_pad_part1 buf1;
@@ -896,10 +917,10 @@ let pad padding n len =
   (* Proof that this is the concatenation of the three parts *)
   let h1 = ST.get () in
   Buffer.no_upd_lemma_2 h0 h1 buf1 buf2 zeros;
-  Seq.lemma_eq_intro (as_seq h1 zeros) (Seq.create (v pad0len) 0uy);
-  assert(as_seq h1 zeros == Seq.create (v pad0len) 0uy);
-  assert(as_seq h1 buf1 == Seq.create 1 0x80uy);
-  assert(as_seq h1 buf2 == Endianness.big_bytes size_len_8 (H128.v encodedlen));
+  Seq.lemma_eq_intro (reveal_sbytes (as_seq h1 zeros)) (Seq.create (v pad0len) 0uy);
+  assert(reveal_sbytes (as_seq h1 zeros) == Seq.create (v pad0len) 0uy);
+  assert(reveal_sbytes (as_seq h1 buf1) == Seq.create 1 0x80uy);
+  assert(reveal_sbytes (as_seq h1 buf2) == Endianness.big_bytes size_len_8 (H128.v encodedlen));
   Lemmas.lemma_sub_append_3 h1 padding 0ul buf1 1ul zeros (1ul +^ pad0len) buf2 (1ul +^ pad0len +^ size_len_8);
   Lemmas.lemma_pad_aux h1 n len buf1 zeros buf2
 
@@ -916,14 +937,14 @@ val update_last:
                   let seq_counter = Seq.slice (as_seq h0 state) (U32.v pos_count_w) (U32.(v pos_count_w + v size_count_w)) in
                   let counter = Seq.index seq_counter 0 in
                   let nb = U64.div len (u32_to_u64 size_block) in
-                  seq_k == Spec.k /\ H64.v counter < (pow2 64 - 2))))
+                  reveal_h64s seq_k == Spec.k /\ H64.v counter < (pow2 64 - 2))))
         (ensures  (fun h0 r h1 -> live h0 state /\ live h0 data /\ live h1 state /\ modifies_1 state h0 h1
                   /\ (let seq_hash_0 = Seq.slice (as_seq h0 state) (U32.v pos_whash_w) (U32.(v pos_whash_w + v size_whash_w)) in
                   let seq_hash_1 = Seq.slice (as_seq h1 state) (U32.v pos_whash_w) (U32.(v pos_whash_w + v size_whash_w)) in
-                  let seq_data = as_seq h0 data in
+                  let seq_data = reveal_sbytes (as_seq h0 data) in
                   let count = Seq.slice (as_seq h0 state) (U32.v pos_count_w) (U32.v pos_count_w + 1) in
-                  let prevlen = U64.(v (Seq.index count 0) * (U32.v size_block)) in
-                  seq_hash_1 == Spec.update_last seq_hash_0 prevlen seq_data)))
+                  let prevlen = H64.((H64.v (Seq.index count 0)) * (U32.v size_block)) in
+                  reveal_h64s seq_hash_1 == Spec.update_last (reveal_h64s seq_hash_0) prevlen seq_data)))
 
 #reset-options "--max_fuel 0  --z3rlimit 200"
 
@@ -936,7 +957,7 @@ let update_last state data len =
   let blocks = Buffer.create (uint8_to_sint8 0uy) (2ul *^ size_block) in
 
   (**) let h0 = ST.get () in
-  (**) assert(as_seq h0 blocks == Seq.create (2 * v size_block) 0uy);
+  (**) assert(reveal_sbytes (as_seq h0 blocks) == Seq.create (2 * v size_block) 0uy);
 
   (* Verification of how many blocks are necessary *)
   (* Threat model. The length are considered public here ! *)
@@ -946,12 +967,12 @@ let update_last state data len =
   in
 
   (**) let h1 = ST.get () in
-  (**) Seq.lemma_eq_intro (as_seq h1 final_blocks)
+  (**) Seq.lemma_eq_intro (reveal_sbytes (as_seq h1 final_blocks))
                           (if U64.(len <^ 112uL) then
                               Seq.create (v size_block) 0uy
                            else Seq.create (2 * v size_block) 0uy);
-  (**) Seq.lemma_eq_intro (as_seq h1 final_blocks) (Seq.create (v nb * v size_block) 0uy);
-  (**) assert(as_seq h1 final_blocks == Seq.create (v nb * v size_block) 0uy);
+  (**) Seq.lemma_eq_intro (reveal_sbytes (as_seq h1 final_blocks)) (Seq.create (v nb * v size_block) 0uy);
+  (**) assert(reveal_sbytes (as_seq h1 final_blocks) == Seq.create (v nb * v size_block) 0uy);
 
   (* Copy the data to the final construct *)
   (* Leakage model : allowed because the length is public *)
@@ -971,8 +992,8 @@ let update_last state data len =
   (**) assert(H64.v n * v size_block + U64.v len < Spec.max_input_len_8);
   (**) assert(length padding = (1 + (Spec.pad0_length (U64.v len)) + v size_len_8));
   (**) assert((length padding + U64.v len) % v size_block = 0);
-  (**) Seq.lemma_eq_intro (as_seq h1 padding) (Seq.create (1 + (Spec.pad0_length (U64.v len)) + v size_len_8) 0uy);
-  (**) assert(as_seq h2 padding == Seq.create (1 + (Spec.pad0_length (U64.v len)) + v size_len_8) 0uy);
+  (**) Seq.lemma_eq_intro (reveal_sbytes (as_seq h1 padding)) (Seq.create (1 + (Spec.pad0_length (U64.v len)) + v size_len_8) 0uy);
+  (**) assert(reveal_sbytes (as_seq h2 padding) == Seq.create (1 + (Spec.pad0_length (U64.v len)) + v size_len_8) 0uy);
   pad padding n len;
 
   (* Proof that final_blocks = data @| padding *)
@@ -981,7 +1002,7 @@ let update_last state data len =
   (**) no_upd_lemma_1 h2 h3 padding data;
   (**) Seq.lemma_eq_intro (as_seq h3 (Buffer.sub final_blocks 0ul (u64_to_u32 len))) (Seq.slice (as_seq h3 final_blocks) 0 (U64.v len));
   (**) no_upd_lemma_1 h2 h3 padding (Buffer.sub final_blocks 0ul (u64_to_u32 len));
-  (**) assert(as_seq h3 data == Seq.slice (as_seq h3 final_blocks) 0 (U64.v len));
+  (**) assert(reveal_sbytes (as_seq h3 data) == Seq.slice (reveal_sbytes (as_seq h3 final_blocks)) 0 (U64.v len));
 
   (**) Seq.lemma_eq_intro (as_seq h3 (Buffer.offset final_blocks (u64_to_u32 len))) (Seq.slice (as_seq h3 final_blocks) (U64.v len) (v nb * v size_block));
   (**) Seq.lemma_eq_intro (as_seq h3 padding) (Seq.slice (as_seq h3 final_blocks) (U64.v len) (v nb * v size_block));
@@ -996,7 +1017,7 @@ let update_last state data len =
   (**) assert(let seq_k = Seq.slice (as_seq h3 state) (U32.v pos_k_w) (U32.(v pos_k_w + v size_k_w)) in
               let seq_counter = Seq.slice (as_seq h3 state) (U32.v pos_count_w) (U32.(v pos_count_w + v size_count_w)) in
               let counter = Seq.index seq_counter 0 in
-              seq_k == Spec.k /\ H64.v counter < (pow2 64 - 2));
+              reveal_h64s seq_k == Spec.k /\ H64.v counter < (pow2 64 - 2));
 
   update_multi state final_blocks nb;
 
@@ -1004,7 +1025,7 @@ let update_last state data len =
   (**) pop_frame()
 
 
-#reset-options "--max_fuel 0  --z3rlimit 10"
+#reset-options "--max_fuel 0  --z3rlimit 20"
 
 [@"substitute"]
 val finish_core:
@@ -1013,8 +1034,8 @@ val finish_core:
   Stack unit
         (requires (fun h0 -> live h0 hash_w /\ live h0 hash))
         (ensures  (fun h0 _ h1 -> live h0 hash_w /\ live h0 hash /\ live h1 hash /\ modifies_1 hash h0 h1
-                  /\ (let seq_hash_w = as_seq h0 hash_w in
-                  let seq_hash = as_seq h1 hash in
+                  /\ (let seq_hash_w = reveal_h64s (as_seq h0 hash_w) in
+                  let seq_hash = reveal_sbytes (as_seq h1 hash) in
                   seq_hash = Spec.words_to_be (U32.v size_hash_w) seq_hash_w)))
 
 [@"substitute"]
@@ -1030,15 +1051,15 @@ val finish:
         (requires (fun h0 -> live h0 state /\ live h0 hash))
         (ensures  (fun h0 _ h1 -> live h0 state /\ live h1 hash /\ modifies_1 hash h0 h1
                   /\ (let seq_hash_w = Seq.slice (as_seq h0 state) (U32.v pos_whash_w) (U32.(v pos_whash_w + v size_whash_w)) in
-                  let seq_hash = as_seq h1 hash in
-                  seq_hash = Spec.finish seq_hash_w)))
+                  let seq_hash = reveal_sbytes (as_seq h1 hash) in
+                  seq_hash = Spec.finish (reveal_h64s seq_hash_w))))
 
 let finish state hash =
   let hash_w = Buffer.sub state pos_whash_w size_whash_w in
   finish_core hash_w hash
 
 
-#reset-options "--max_fuel 0  --z3rlimit 10"
+#reset-options "--max_fuel 0  --z3rlimit 20"
 
 val hash:
   hash :uint8_p {length hash = v size_hash} ->
@@ -1047,8 +1068,8 @@ val hash:
   Stack unit
         (requires (fun h0 -> live h0 hash /\ live h0 input))
         (ensures  (fun h0 _ h1 -> live h0 input /\ live h0 hash /\ live h1 hash /\ modifies_1 hash h0 h1
-                  /\ (let seq_input = as_seq h0 input in
-                  let seq_hash = as_seq h1 hash in
+                  /\ (let seq_input = reveal_sbytes (as_seq h0 input) in
+                  let seq_hash = reveal_sbytes (as_seq h1 hash) in
                   seq_hash == Spec.hash seq_input)))
 
 #reset-options "--max_fuel 0  --z3rlimit 50"
